StmtRel.thy
@@ -477,7 +477,7 @@ lemma field_assign_rel:
     Rext: "Rext = (\<lambda> \<omega>def \<omega> ns. \<omega>def = \<omega> \<and> R \<omega> ns)"  and
     RcvWfRel: "expr_wf_rel Rext ctxt_vpr StateCons P ctxt rcv_vpr \<gamma> \<gamma>1" and
     RhsWfRel: "expr_wf_rel Rext ctxt_vpr StateCons P ctxt rhs_vpr \<gamma>1 \<gamma>2" and
-    WriteableLocRel: "wf_rel_fieldacc get_writeable_locs Rext ctxt_vpr StateCons P ctxt rcv_vpr f_vpr 
+    WriteableLocRel: "wf_rel_fieldacc get_writeable_locs Rext Rext ctxt_vpr StateCons P ctxt rcv_vpr f_vpr 
                  \<gamma>2 
                  ((BigBlock name ((Lang.Assign h_bpl h_upd_bpl)#cs) str tr), cont)" and 
                    "h_bpl = heap_var Tr" and
@@ -652,7 +652,7 @@ lemma field_assign_rel_inst:
     Rext: "Rext = (\<lambda> \<omega>def \<omega> ns. \<omega>def = \<omega> \<and> R \<omega> ns)"  and
     RcvWfRel: "expr_wf_rel Rext ctxt_vpr StateCons P ctxt rcv_vpr \<gamma> \<gamma>1" and
     RhsWfRel: "expr_wf_rel Rext ctxt_vpr StateCons P ctxt rhs_vpr \<gamma>1 \<gamma>2" and
-    WriteableLocRel: "wf_rel_fieldacc get_writeable_locs Rext ctxt_vpr StateCons P ctxt rcv_vpr f_vpr 
+    WriteableLocRel: "wf_rel_fieldacc get_writeable_locs Rext Rext ctxt_vpr StateCons P ctxt rcv_vpr f_vpr 
                  \<gamma>2 
                  ((BigBlock name ((Lang.Assign h_bpl h_upd_bpl)#cs) str tr), cont)" and 
                    "h_bpl = heap_var Tr" and
